More work on the overlay semantics

theories/overlay.v
@@ -1,14 +1,39 @@
 From iris.algebra Require Import base.
 From iris.program_logic Require Import language ectx_language ectxi_language.
-From stdpp Require Import gmap fin_maps list.
+From stdpp Require Import gmap fin_maps list finite.
 From cap_machine Require Export addr_reg machine_base machine_parameters.
+
+(* TODO: move to addr_reg.v *)
+
+Definition all_registers: list RegName :=
+  [R 0 eq_refl; R 1 eq_refl; R 2 eq_refl; R 3 eq_refl; R 4 eq_refl; R 5 eq_refl;
+   R 6 eq_refl; R 7 eq_refl; R 8 eq_refl; R 9 eq_refl; R 10 eq_refl; R 11 eq_refl;
+   R 12 eq_refl; R 13 eq_refl; R 14 eq_refl; R 15 eq_refl; R 16 eq_refl; R 17 eq_refl;
+   R 18 eq_refl; R 19 eq_refl; R 20 eq_refl; R 21 eq_refl; R 22 eq_refl; R 23 eq_refl;
+   R 24 eq_refl; R 25 eq_refl; R 26 eq_refl; R 27 eq_refl; R 28 eq_refl; R 29 eq_refl;
+   R 30 eq_refl; R 31 eq_refl; PC].
+
+Global Instance RegName_finite: Finite RegName.
+Proof.
+  refine {| enum := all_registers;
+            NoDup_enum := _;
+            elem_of_enum := _ |}.
+  { repeat (econstructor; [set_solver|]).
+    econstructor. }
+  { destruct x; [set_solver|].
+    do 32 (destruct n as [|n]; [rewrite (@Eqdep_dec.eq_proofs_unicity bool ltac:(decide equality) _ _ fin (eq_refl _)); set_solver|]).
+    simpl in fin. discriminate. }
+Qed.
 
 Inductive Cap: Type :=
 | Regular: machine_base.Cap -> Cap (* Regular capabilities *)
 | Stk: nat -> Perm -> Addr -> Addr -> Addr -> Cap (* Stack derived capabilities *)
 | Ret: nat -> Addr -> Addr -> Addr -> Cap. (* Return capabilities *)
 
-Coercion Regular : machine_base.Cap >-> Cap.
+Instance cap_eq_dec : EqDecision Cap.
+Proof. solve_decision. Defined.
+Instance word_eq_dec : EqDecision Word.
+Proof. solve_decision. Defined.
 
 Definition Word := (Z + Cap)%type.
 
@@ -214,6 +239,32 @@ Inductive isCorrectPC: Word → Prop :=
       p = RX \/ p = RWX \/ p = RWLX →
       isCorrectPC (inr (Stk d p b e a)).
 
+Lemma isCorrectPC_dec:
+  forall w, { isCorrectPC w } + { not (isCorrectPC w) }.
+Proof.
+  destruct w.
+  - right. red; intros H. inversion H.
+  - destruct c.
+    + destruct c as ((((p & g) & b) & e) & a).
+      case_eq (match p with RX | RWX | RWLX => true | _ => false end); intros.
+      * destruct (Addr_le_dec b a).
+        { destruct (Addr_lt_dec a e).
+          { left. econstructor; simpl; eauto. by auto.
+            destruct p; naive_solver. }
+          { right. red; intro HH. inversion HH; subst. solve_addr. } }
+        { right. red; intros HH; inversion HH; subst. solve_addr. }
+      * right. red; intros HH; inversion HH; subst. naive_solver.
+    + case_eq (match p with RX | RWX | RWLX => true | _ => false end); intros.
+      * destruct (Addr_le_dec a a1).
+        { destruct (Addr_lt_dec a1 a0).
+          { left. econstructor; simpl; eauto. by auto.
+            destruct p; naive_solver. }
+          { right. red; intro HH. inversion HH; subst. solve_addr. } }
+        { right. red; intros HH; inversion HH; subst. solve_addr. }
+      * right. red; intros HH; inversion HH; subst. naive_solver.
+    + right. red; intros H. inversion H.
+Qed.
+
 Section opsem.
   Context `{MachineParameters}.
 
@@ -226,7 +277,7 @@ Section opsem.
       | inr (Ret d b e a) => match jmp_ret d (callstack φ) with
                             | None => (Failed, φ)
                             | Some ((reg', m'), cs) => (NextI, (merge (fun a b => match a with Some _ => a | _ => b end) reg' (reg φ), mem φ, m', cs))
-                                                        (* TODO: this is not safe if registers are not cleared beforehands *)
+                                                        (* TODO: this is wrong *)
                       end
       | _ => let φ' :=  (update_reg φ PC (updatePcPerm (RegLocate (reg φ) r))) in (NextI, φ')
       end
@@ -766,18 +817,124 @@ Section opsem.
       end
     end.
 
+  Definition decodeInstrW' (w: Word) :=
+    match w with
+    | inl n => decodeInstrW (inl n)
+    | inr _ => Fail
+    end.
+
+  Definition rclear_instrs (r : list RegName): list Word := map (λ r_i, inl (encodeInstr (Mov r_i (inl 0%Z)))) r.
+
+  Definition return_instrs r := rclear_instrs (list_difference all_registers [PC; r]) ++ [inl (encodeInstr (Jmp r))].
+
+  Lemma return_instrs_length:
+    forall r, r <> PC -> length (return_instrs r) = RegNum + 1.
+  Proof.
+    destruct r; try congruence.
+    intros. rewrite /return_instrs /rclear_instrs.
+    rewrite app_length.
+    do 32 (destruct n as [|n]; [simpl; reflexivity|]).
+    simpl in fin. discriminate.
+  Qed.
+
   Inductive step: Conf → Conf → Prop :=
   | step_exec_fail:
       forall φ,
         not (isCorrectPC ((reg φ) !r! PC)) →
         step (Executable, φ) (Failed, φ)
   | step_exec_instr:
-      forall φ p g b e a i c,
+      forall φ p g b e a i c rd rb re ra,
         RegLocate (reg φ) PC = inr (Regular ((p, g), b, e, a)) ->
         isCorrectPC ((reg φ) !r! PC) →
-        decodeInstrW ((mem φ) !m! a) = i →
+        decodeInstrW' ((mem φ) !m! a) = i →
         exec i φ = c →
+        ~ (exists r, r <> PC /\ (reg φ !r! r = inr (Ret rd rb re ra)) /\
+                forall i, (i <= RegNum)%nat ->
+                     exists a_i, (a + i)%a = Some a_i /\ (return_instrs r) !! i = Some ((mem φ) !m! a_i)) ->
+        step (Executable, φ) (c.1, c.2)
+  | step_exec_instr':
+      forall φ d p b e a i c m,
+        RegLocate (reg φ) PC = inr (Stk d p b e a) ->
+        isCorrectPC ((reg φ) !r! PC) →
+        stack d ((reg φ, stk φ)::(callstack φ)) = Some m ->
+        decodeInstrW' (m !m! a) = i →
+        exec i φ = c →
+        step (Executable, φ) (c.1, c.2)
+  | step_exec_return:
+      forall φ p g b e a a' c rd rb re ra,
+        RegLocate (reg φ) PC = inr (Regular ((p, g), b, e, a)) ->
+        isCorrectPC ((reg φ) !r! PC) →
+        (a + RegNum)%a = Some a' ->
+        (a' < e)%a ->
+        (exists r, r <> PC /\ (reg φ !r! r = inr (Ret rd rb re ra)) /\
+             forall i, (i <= RegNum)%nat ->
+                  exists a_i, (a + i)%a = Some a_i /\ (return_instrs r) !! i = Some ((mem φ) !m! a_i)) ->
+        c = match jmp_ret rd (callstack φ) with
+            | None => (Failed, φ) (* Should never happen ? *)
+            | Some ((reg', m'), cs) => (NextI, (merge (fun a b => match a with Some _ => a | _ => Some (inl 0%Z) end) reg' (reg φ), mem φ, m', cs))
+            end ->
         step (Executable, φ) (c.1, c.2).
+  (* TODO: add call, tailcall semantics and PC = Stk capability version *)
+
+  Lemma is_return_dec:
+    forall reg mem rd rb re ra a,
+      {exists r, r <> PC /\ (reg !r! r = inr (Ret rd rb re ra)) /\
+             forall i, (i <= RegNum)%nat ->
+                  exists a_i, (a + i)%a = Some a_i /\ (return_instrs r) !! i = Some ((mem) !m! a_i)} +
+      {~ exists r, r <> PC /\ (reg !r! r = inr (Ret rd rb re ra)) /\
+                forall i, (i <= RegNum)%nat ->
+                     exists a_i, (a + i)%a = Some a_i /\ (return_instrs r) !! i = Some ((mem) !m! a_i)}.
+  Proof.
+    intros. eapply exists_dec. intros.
+    destruct (reg_eq_dec x PC).
+    - right. red; intros (A & B & C). congruence.
+    - assert ({reg0 !r! x = inr (Ret rd rb re ra)} + {reg0 !r! x <> inr (Ret rd rb re ra)}) by solve_decision.
+      destruct H0.
+      + assert ({∀ i : nat, i ≤ RegNum → ∃ a_i : Addr, (a + i)%a = Some a_i ∧ return_instrs x !! i = Some (mem0 !m! a_i)} + {~∀ i : nat, i ≤ RegNum → ∃ a_i : Addr, (a + i)%a = Some a_i ∧ return_instrs x !! i = Some (mem0 !m! a_i)}).
+        { assert ((∀ i : nat, i ≤ RegNum → ∃ a_i : Addr, (a + i)%a = Some a_i ∧ return_instrs x !! i = Some (mem0 !m! a_i)) <-> (forall i: fin (S RegNum), ∃ a_i : Addr, (a + (fin_to_nat i))%a = Some a_i ∧ return_instrs x !! (fin_to_nat i) = Some (mem0 !m! a_i))).
+        { split; intros.
+          - eapply H0. generalize (fin_to_nat_lt i). lia.
+          - assert (i < S RegNum) by lia.
+            generalize (H0 (nat_to_fin H2)).
+            rewrite fin_to_nat_to_fin. auto. }
+        assert ({forall i: fin (S RegNum), ∃ a_i : Addr, (a + (fin_to_nat i))%a = Some a_i ∧ return_instrs x !! (fin_to_nat i) = Some (mem0 !m! a_i)} + {~ forall i: fin (S RegNum), ∃ a_i : Addr, (a + (fin_to_nat i))%a = Some a_i ∧ return_instrs x !! (fin_to_nat i) = Some (mem0 !m! a_i)}).
+        { eapply forall_dec. intros.
+          case_eq (a + x0)%a; intros.
+          - assert ({return_instrs x !! (fin_to_nat x0) = Some (mem0 !m! a0)} + {~ return_instrs x !! (fin_to_nat x0) = Some (mem0 !m! a0)}). decide equality. decide equality. apply Z_eq_dec. apply cap_eq_dec.
+            destruct H2.
+            + left; eauto.
+            + right. red; intros.
+              destruct H2 as [y [A B]]. congruence.
+          - right. red; intros. destruct H2 as [y [A B]]. congruence. }
+        destruct H1.
+          - left. intros. assert (i < S RegNum) by lia.
+            generalize (e0 (nat_to_fin H2)). rewrite fin_to_nat_to_fin. eauto.
+          - right. red; intros. eapply n0. intros. eapply H1. generalize (fin_to_nat_lt i). lia. }
+        destruct H0.
+        * left; auto.
+        * right. red; intros (A & B & C). congruence.
+      + right. red; intros (A & B & C). congruence.
+  Qed.
+
+  Lemma normal_always_step:
+    forall φ, exists cf φ', step (Executable, φ) (cf, φ').
+  Proof.
+    intros. destruct (isCorrectPC_dec (RegLocate (reg φ) PC)).
+    - inversion i; subst.
+      + do 2 eexists; eapply step_exec_instr; eauto.
+
+    - exists Failed, φ. constructor 1; eauto.
+  Qed.
+
+  Lemma step_deterministic:
+    forall c1 c2 c2' σ1 σ2 σ2',
+      step (c1, σ1) (c2, σ2) →
+      step (c1, σ1) (c2', σ2') →
+      c2 = c2' ∧ σ2 = σ2'.
+  Proof.
+    intros * H1 H2; split; inv H1; inv H2; auto; try congruence.
+  Qed.
+
 
 
 
